Extensions/ShallowEmbedded/MonoPredicateStable.v
@@ -1,0 +1,73 @@
+Require Import Logic.lib.Ensembles_ext.
+Require Import Logic.GeneralLogic.Base.
+Require Import Logic.MinimunLogic.Syntax.
+Require Import Logic.PropositionalLogic.Syntax.
+Require Import Logic.ModalLogic.Syntax.
+Require Import Logic.MinimunLogic.ProofTheory.Normal.
+Require Import Logic.MinimunLogic.ProofTheory.Minimun.
+Require Import Logic.PropositionalLogic.ProofTheory.Intuitionistic.
+Require Import Logic.ModalLogic.ProofTheory.ModalLogic.
+Require Import Logic.Extensions.ProofTheory.Stable.
+Require Import Logic.GeneralLogic.KripkeModel.
+Require Import Logic.ModalLogic.Model.KripkeModel.
+Require Import Logic.ModalLogic.Model.OrderedKripkeModel.
+Require Import Logic.SeparationLogic.Model.SeparationAlgebra.
+Require Import Logic.SeparationLogic.Model.OrderedSA.
+Require Import Logic.Extensions.Semantics.SemanticStable.
+Require Import Logic.ModalLogic.Semantics.Flat.
+Require Import Logic.SeparationLogic.Semantics.FlatSemantics.
+Require Import Logic.Extensions.Sound.StableSound.
+Require Import Logic.GeneralLogic.ShallowEmbedded.MonoPredicateAsLang.
+Require Import Logic.PropositionalLogic.ShallowEmbedded.MonoPredicatePropositionalLogic.
+Require Import Logic.ModalLogic.ShallowEmbedded.MonoPredicateModalLogic.
+Require Import Logic.SeparationLogic.ShallowEmbedded.MonoPredicateSeparationLogic.
+
+Instance MonoPred_stableSM (A: Type) {R1: KI.Relation A} {kiM: KripkeIntuitionisticModel A} {R2: SS.Relation A}: @SemanticStable (MonoPred_L A) (Build_Model A) (unit_kMD _) tt R2 (MonoPred_SM A).
+Proof.
+  refine (Build_SemanticStable _ _ _ _ _ _ (fun x => Semantics.stable (@Kdenotation _ _ (unit_kMD _) tt _ x)) _).
+  intros. reflexivity.
+Defined.
+
+Instance MonoPred_pstable (A: Type) {R1: KI.Relation A} {kiM: KripkeIntuitionisticModel A} {R2: SS.Relation A} {KI_bis_R2: KripkeIntuitionisticBisStable A}: PropositionalStable (MonoPred_L A) (MonoPred_Gamma A) (fun x => Semantics.stable (@Kdenotation _ (Build_Model A) (unit_kMD _) tt _ x)).
+Proof.
+  constructor.
+  + intros x y.
+    exact (@Sound_KripkeIntuitionistic.sound_impp_stable (MonoPred_L A) _ _ (Build_Model A) (unit_kMD _) tt R1 _ _ (MonoPred_SM A) (MonoPred_kiSM A) (MonoPred_stableSM A) x y).
+  + intros x y.
+    exact (@Sound_KripkeIntuitionistic.sound_andp_stable (MonoPred_L A) _ _ (Build_Model A) (unit_kMD _) tt R1 _ (MonoPred_SM A) (MonoPred_kiSM A) (MonoPred_stableSM A) x y).
+  + intros x y.
+    exact (@Sound_KripkeIntuitionistic.sound_orp_stable (MonoPred_L A) _ _ (Build_Model A) (unit_kMD _) tt R1 _ (MonoPred_SM A) (MonoPred_kiSM A) (MonoPred_stableSM A) x y).
+  + exact (@Sound_KripkeIntuitionistic.sound_falsep_stable (MonoPred_L A) _ _ (Build_Model A) (unit_kMD _) tt R1 _ (MonoPred_SM A) (MonoPred_kiSM A) (MonoPred_stableSM A)).
+  + hnf; intros x y.
+    exact (@Sound_KripkeIntuitionistic.sound_stable_proper_iffp (MonoPred_L A) _ _ (Build_Model A) (unit_kMD _) tt R1 _ _ (MonoPred_SM A) (MonoPred_kiSM A) (MonoPred_stableSM A) x y).
+Qed.
+
+Instance MonoPred_mstable (A: Type) {R1: KI.Relation A} {kiM: KripkeIntuitionisticModel A} {R2: KM.Relation A} {R3: SS.Relation A} {ukmM: UpwardsClosedOrderedKripkeModel A} {KM_bis_R3: KripkeModalBisStable A}: ModalStable (MonoPred_L A) (MonoPred_Gamma A) (fun x => Semantics.stable (@Kdenotation _ (Build_Model A) (unit_kMD _) tt _ x)).
+Proof.
+  constructor.
+  intros x.
+  exact (@Sound_KripkeIntuitionistic.sound_boxp_stable (MonoPred_L A) _ _ _ (Build_Model A) (unit_kMD _) tt R1 _ _ _ (MonoPred_SM A) (MonoPred_fmSM A) (MonoPred_stableSM A) x).
+Qed.
+
+Instance MonoPred_MAS (A: Type) {R1: KI.Relation A} {kiM: KripkeIntuitionisticModel A} {R2: KM.Relation A} {R3: SS.Relation A} {ukmM: UpwardsClosedOrderedKripkeModel A} {KM_abs_R3: KripkeModalAbsorbStable A}: ModalAbsorbStable (MonoPred_L A) (MonoPred_Gamma A) (fun x => Semantics.stable (@Kdenotation _ (Build_Model A) (unit_kMD _) tt _ x)).
+Proof.
+  constructor.
+  intros x.
+  exact (@Sound_KripkeIntuitionistic.sound_boxp_absorb_stable (MonoPred_L A) _ _ _ (Build_Model A) (unit_kMD _) tt R1 _ _ _ (MonoPred_SM A) (MonoPred_kiSM A) (MonoPred_fmSM A) (MonoPred_stableSM A) x).
+Qed.
+
+Instance MonoPred_sstable (A: Type) {R1: KI.Relation A} {kiM: KripkeIntuitionisticModel A} {J: Join A} {SA: SeparationAlgebra A} {uSA: UpwardsClosedSeparationAlgebra A} {dSA: DownwardsClosedSeparationAlgebra A} {R2: SS.Relation A} {SA_bis_R2: SeparationAlgebraBisStable A}: SeparationStable (MonoPred_L A) (MonoPred_Gamma A) (fun x => Semantics.stable (@Kdenotation _ (Build_Model A) (unit_kMD _) tt _ x)).
+Proof.
+  constructor.
+  + intros x y.
+    exact (@Sound_KripkeIntuitionistic.sound_sepcon_stable (MonoPred_L A) _ _ _ (Build_Model A) (unit_kMD _) tt R1 _ _ _ (MonoPred_SM A) (MonoPred_fsSM A) (MonoPred_stableSM A) x y).
+  + intros x y.
+    exact (@Sound_KripkeIntuitionistic.sound_wand_stable (MonoPred_L A) _ _ _ (Build_Model A) (unit_kMD _) tt R1 _ _ _ (MonoPred_SM A) (MonoPred_fsSM A) (MonoPred_stableSM A) x y).
+Qed.
+
+Instance MonoPred_SAS (A: Type) {R1: KI.Relation A} {kiM: KripkeIntuitionisticModel A} {J: Join A} {SA: SeparationAlgebra A} {uSA: UpwardsClosedSeparationAlgebra A} {dSA: DownwardsClosedSeparationAlgebra A} {R2: SS.Relation A} {SA_abs_R2: SeparationAlgebraAbsorbStable A}: SeparationAbsorbStable (MonoPred_L A) (MonoPred_Gamma A) (fun x => Semantics.stable (@Kdenotation _ (Build_Model A) (unit_kMD _) tt _ x)).
+Proof.
+  constructor.
+  intros x y z.
+  exact (@Sound_KripkeIntuitionistic.sound_stable_andp_sepcon1 (MonoPred_L A) _ _ _ (Build_Model A) (unit_kMD _) tt R1 _ _ _ (MonoPred_SM A) (MonoPred_kiSM A) (MonoPred_fsSM A) (MonoPred_stableSM A) x y z).
+Qed.
